\begin{answer}
    \begin{align*}
        p(t^{(i)}= 1|x^{(i)}) &= \frac{p(x^{(i)} | t^{(i)}= 1) p(t^{(i)}= 1)}{p(x^{(i)})}\\
        &= \frac{p(x^{(i)} | t^{(i)}= 1)p(y^{(i)}=1|t^{(i)}=1) p(t^{(i)}= 1)}{p(x^{(i)}) p(y^{(i)}=1|t^{(i)}=1)}\\
         &= \frac{p(y^{(i)}=1 , x^{(i)} |t^{(i)}=1) p(t^{(i)}= 1)}{p(x^{(i)}) p(y^{(i)}=1|t^{(i)}=1)}\text{\ \ \ Because $x$ and $y$ independent}\\
         &= \frac{p(y^{(i)}=1|x^{(i)}) p(x^{(i)}| t^{(i)}= 1) p(t^{(i)}= 1)}{p(x^{(i)}) p(y^{(i)}=1|t^{(i)}=1)}\text{\ \ \ Chain rule}\\
         &= \frac{p(y^{(i)}=1|x^{(i)}) p(x^{(i)})}{p(x^{(i)}) p(y^{(i)}=1|t^{(i)}=1)}\\
         &= \frac{p(y^{(i)}=1|x^{(i)}) }{ p(y^{(i)}=1|t^{(i)}=1)}
    \end{align*}
    So $\alpha = p(y^{(i)}=1|t^{(i)}=1)$
\end{answer}
